language_formalisation/syntax/term_syntax.v
@@ -1,0 +1,83 @@
+Require Import Bool List ZArith Int String.
+
+Definition var_id := string.
+Definition op_id := string.
+Definition int := Z.t.
+Definition eq_id := string_dec.
+
+Inductive val : Type :=
+| Var : string -> val
+| Unit : val
+| Int : Z.t -> val
+| Inl : val -> val
+| Inr : val -> val
+| Pair : val -> val -> val
+| Fun : var_id -> comp -> val
+| Handler : var_id -> comp -> hcases -> val
+with comp : Type :=
+| Ret : val -> comp
+| PairMatch : val -> var_id * var_id -> comp -> comp
+| SumMatch : val -> var_id -> comp -> var_id -> comp -> comp
+| App : val -> val -> comp
+| Op : op_id -> val -> var_id -> comp -> comp
+| LetRec : var_id -> var_id -> comp -> comp -> comp
+| DoBind : var_id -> comp -> comp -> comp
+| Handle : val -> comp -> comp
+with hcases : Type :=
+| Empty : hcases
+| OpCases : hcases -> op_id -> var_id -> var_id -> comp -> hcases.
+
+(* NOT CAPTURE AVOIDING!!! *)
+Fixpoint vsubst (sub : var_id * val) (v : val) :=
+  (* v [id |-> sv] *)
+  let (s_id, s_v) := sub in
+  match v with
+  | Var id => if eq_id id s_id then s_v else v
+  | Unit => v
+  | Int n => v
+  | Inl v' => vsubst sub v'
+  | Inr v' => vsubst sub v'
+  | Pair v1 v2 => Pair (vsubst sub v1) (vsubst sub v2)
+  | Fun id c => if eq_id id s_id then v else Fun id (csubst sub c) 
+  | Handler ret_id c h => 
+      if eq_id ret_id s_id then Handler ret_id c (hsubst sub h)
+      else Handler ret_id (csubst sub c) (hsubst sub h)
+  end
+with csubst (sub : var_id * val) (c : comp) :=
+  (* c [id |-> sv] *)
+  let (s_id, s_v) := sub in
+  match c with
+  | Ret v => Ret (vsubst sub v)
+  | PairMatch v (id1, id2) c' => 
+      if eq_id id1 s_id then c
+      else if eq_id id2 s_id then c
+      else PairMatch (vsubst sub v) (id1, id2) (csubst sub c')
+  | SumMatch v idl cl idr cr =>
+      let cl' := if eq_id idl s_id then cl else csubst sub cl in
+      let cr' := if eq_id idr s_id then cr else csubst sub cr in
+      SumMatch (vsubst sub v) idl cl' idr cr'
+  | App vf vx => App (vsubst sub vf) (vsubst sub vx)
+  | Op op_id v_arg id k =>
+      let k' := if eq_id id s_id then k else csubst sub k in
+      Op op_id (vsubst sub v_arg) id k'
+  | LetRec f_id x_id c1 c2 =>
+      if eq_id f_id s_id then c
+      else if eq_id x_id s_id then c
+      else LetRec f_id x_id (csubst sub c1) (csubst sub c2)
+  | DoBind x_id c1 c2 =>
+      if eq_id x_id s_id then DoBind x_id (csubst sub c1) c2
+      else DoBind x_id (csubst sub c1) (csubst sub c2)
+  | Handle v c' => Handle (vsubst sub v) (csubst sub c')
+  end
+with hsubst (sub : var_id * val) (h : hcases) :=
+  (* c [id |-> sv] *)
+  let (s_id, s_v) := sub in
+  match h with
+  | Empty => h
+  | OpCases h' op_id x_id k_id c_op =>
+      let c_op' := 
+        if eq_id x_id s_id then c_op
+        else if eq_id k_id s_id then c_op
+      else csubst sub c_op in
+      OpCases (hsubst sub h') op_id x_id k_id c_op'
+  end.
